redefined domination lattice by ListSet.
The lattice by FSet is good for the fsetdec tactics, but makes inductive
principles over FSet hard to use. The problem is FSet interface is not
affected by the order of its underlying elememts, so if we use its
'fold' to compute anything, the fold's ind-rule has to ensure this
invariant by showing that relative properties are instances of
'Equivalence'.

The ListSet impl fixed the problem, while we need to define new tactics
to automate proofs.



git-svn-id: https://webdav.seas.upenn.edu/svn/sol/vol@2950 eef5ea85-cc2e-0410-bd84-0fae1f012da8

src/ssa/ssa_analysis.v
@@ -20,8 +20,113 @@ Require Import Maps.
 Require Import Lattice.
 Require Import Iteration.
 Require Import Kildall.
+Require Import ListSet.
 
 Export LLVMlib.
+
+Module AtomSet.
+
+  Definition set_eq A (l1 l2:list A) := incl l1 l2 /\ incl l2 l1.
+
+  Lemma set_eq_dec : forall (l1 l2:set atom), 
+    {set_eq _ l1 l2} + {~ set_eq _ l1 l2}.
+  Proof.
+  induction l1; intros.
+    destruct l2.
+      left. split; intros a H; eauto.
+      right. intro J. destruct J. 
+        assert (J:=@H0 a). 
+        apply J; simpl; auto. 
+
+    destruct l2.
+      right. intro J. destruct J. 
+        assert (J:=@H a). 
+        apply J; simpl; auto. 
+
+        destruct (@IHl1 l2) as [[J1 J2] | J].
+          destruct (eq_atom_dec a a0); subst.
+            left.        
+            split; intros a H; simpl in *; destruct H as [H | H]; auto.
+      
+            destruct(@in_dec _ eq_atom_dec a l2) as [J3 | J3].     
+              destruct(@in_dec _ eq_atom_dec a0 l1) as [J4 | J4].     
+                left. 
+                split; intros a' H; simpl in *; destruct H as [H | H]; 
+                  subst; auto.
+
+                right.
+                intros [J5 J6].
+                assert (J:=@J6 a0).
+                destruct J; simpl; auto.
+
+              right.
+              intros [J5 J6].
+              assert (J:=@J5 a).
+              destruct J; simpl; auto.
+   (* it is easier to prove uniq lists. *)
+  Admitted.
+
+  Lemma set_eq_refl : forall x, set_eq atom x x.  
+    split; apply incl_refl.
+  Qed.
+
+  Lemma set_eq_sym: forall x y, set_eq atom x y -> set_eq atom y x.
+  Proof.
+    intros x y J.
+    destruct J as [J1 J2]. split; auto.
+  Qed.
+  
+  Lemma set_eq_trans: forall x y z, 
+    set_eq atom x y -> set_eq atom y z -> set_eq atom x z.
+  Proof.
+    intros x y z J1 J2.
+    destruct J1 as [J11 J12].
+    destruct J2 as [J21 J22].
+    split; eapply incl_tran; eauto.
+  Qed.
+
+  Lemma incl_empty_inv : forall x, 
+    incl x (empty_set _) -> x = empty_set atom.
+  Proof.
+    destruct x; intro J; auto.
+      assert (J1:=J a).
+      contradict J1; simpl; auto.
+  Qed.
+
+  Lemma set_eq_empty_inv : forall x, 
+    set_eq atom x (empty_set _) -> x = empty_set _.
+  Proof.
+    destruct x; intro J; auto.
+      destruct J as [J1 J2].
+      assert (J:=J1 a).
+      contradict J; simpl; auto.
+  Qed.
+
+  Lemma incl_set_eq_left : forall x1 x2 y,
+    set_eq atom x1 x2 -> incl x1 y -> incl x2 y.
+  Proof.
+    intros x1 x2 y [J1 J2] Hincl.
+    eapply incl_tran; eauto.
+  Qed.
+
+  Lemma set_eq__incl : forall x1 x2, set_eq atom x1 x2 -> incl x1 x2.
+  Proof.
+    intros x1 x2 J.
+    destruct J; auto.
+  Qed.
+
+  Lemma incl_set_eq_both : forall x1 x2 y1 y2,
+    set_eq atom x1 x2 -> 
+    set_eq atom y1 y2 -> 
+    incl x1 y1 -> incl x2 y2.
+  Proof.
+    intros x1 x2 y1 y2 [J1 J2] [J3 J4] J5.
+    apply incl_tran with (m:=y1); auto.
+    apply incl_tran with (m:=x1); auto.
+  Qed.
+
+
+End AtomSet.
 
 (** * Domination analysis *)
 
@@ -32,13 +137,16 @@ Export LLVMlib.
   the approximations. *)
 
 Module Dominators.
+ 
+  Export AtomSet.
+
   Section VarBoundSec.
 
-  Variable bound:atoms.
+  Variable bound:set atom.
 
   Record BoundedSet := mkBoundedSet {
-    bs_contents : atoms;
-    bs_bound : bs_contents [<=] bound
+    bs_contents : set atom;
+    bs_bound : incl bs_contents bound
   }.
 
   Definition t := BoundedSet.
@@ -46,30 +154,30 @@ Module Dominators.
   Definition eq (x y: t) :=
     let '(mkBoundedSet cx _) := x in
     let '(mkBoundedSet cy _) := y in
-    cx [=] cy.
+    set_eq _ cx cy.
 
   Definition eq_refl: forall x, eq x x. 
   Proof.
     unfold eq. intro x. destruct x.
-    fsetdec.
+    apply set_eq_refl.
   Qed.
 
   Definition eq_sym: forall x y, eq x y -> eq y x.
   Proof.
     unfold eq. intros x y J. destruct x. destruct y.
-    fsetdec.
+    apply set_eq_sym; auto.
   Qed.
-  
+ 
   Definition eq_trans: forall x y z, eq x y -> eq y z -> eq x z.
   Proof.
     unfold eq. intros x y z J1 J2. destruct x. destruct y. destruct z.
-    fsetdec.
+    eapply set_eq_trans; eauto.
   Qed.
 
   Lemma eq_dec: forall (x y: t), {eq x y} + {~ eq x y}.
   Proof.
     unfold eq. destruct x. destruct y.
-    apply AtomSetImpl.eq_dec.
+    apply set_eq_dec.
   Qed.
 
   Definition beq (x y: t) := if eq_dec x y then true else false.
@@ -82,16 +190,16 @@ Module Dominators.
   Definition sub (x y: t) :=
     let '(mkBoundedSet cx _) := x in
     let '(mkBoundedSet cy _) := y in
-    cx [<=] cy.
+    incl cx cy.
 
-  Program Definition top : t := mkBoundedSet {} _.
+  Program Definition top : t := mkBoundedSet (empty_set atom) _.
   Next Obligation.
-    fsetdec.
+    intros a H. inversion H.
   Qed.
 
   Program Definition bot : t := mkBoundedSet bound _.
   Next Obligation.
-    fsetdec.
+    apply incl_refl.
   Qed.
 
   Definition ge (x y: t) : Prop := eq x top \/ eq y bot \/ sub x y.
@@ -99,66 +207,98 @@ Module Dominators.
   Lemma ge_refl: forall x y, eq x y -> ge x y.
   Proof.
     unfold ge, eq, sub. destruct x, y. simpl.
-    intro J. right. right. fsetdec.
+    intro J. right. right. destruct J; auto.
   Qed.
+
   Lemma ge_trans: forall x y z, ge x y -> ge y z -> ge x z.
   Proof.
     unfold ge, eq, sub. destruct x, y, z. simpl.
     intros J1 J2.
     destruct J1 as [J11 | [J12 | J13]]; try auto.
       destruct J2 as [J21 | [J22 | J23]]; try auto.
-        assert (bound [=] empty) as EQ by fsetdec.
-        left. fsetdec.
-        right. left. fsetdec.
+        assert (set_eq _ bound (empty_set atom)) as EQ.
+          eapply set_eq_trans with (y:=bs_contents1); eauto using set_eq_sym.
+        left. 
+        apply set_eq_empty_inv in EQ; subst.
+        apply incl_empty_inv in bs_bound0; subst.
+        apply set_eq_refl.
+
+        right. left. 
+        eapply incl_set_eq_left in J23; eauto.
+        split; auto.
+
       destruct J2 as [J21 | [J22 | J23]]; try auto.
-        left. fsetdec.
-        right. right. fsetdec.
+        left. 
+        apply set_eq_empty_inv in J21; subst.
+        apply incl_empty_inv in J13; subst.
+        apply set_eq_refl.
+
+        right. right. eapply incl_tran; eauto.
   Qed.
+
   Lemma ge_compat: forall x x' y y', eq x x' -> eq y y' -> ge x y -> ge x' y'.
   Proof.
     unfold ge, eq, sub. destruct x, x', y, y'. simpl in *. 
     intros J1 J2 J3.
     destruct J3 as [J31 | [J32 | J33]].
-      left. fsetdec.
-      right. left. fsetdec.
-      right. right. fsetdec.
+      left. eapply set_eq_trans with (y:=bs_contents0); eauto using set_eq_sym.
+      right. left. 
+        eapply set_eq_trans with (y:=bs_contents2); eauto using set_eq_sym.
+      right. right. eapply incl_set_eq_both; eauto. 
   Qed.
+
   Lemma ge_bot: forall x, ge x bot.
   Proof.
-    unfold ge, eq, sub. destruct x. simpl. right. left. fsetdec.
+    unfold ge, eq, sub. destruct x. simpl. right. left. apply set_eq_refl.
   Qed.
+
   Lemma ge_top: forall x, ge top x.
   Proof.
-    unfold ge, eq, sub. destruct x. simpl. left. fsetdec.
+    unfold ge, eq, sub. destruct x. simpl. left. apply set_eq_refl.
   Qed.
+
   Program Definition lub (x y: t) : t :=
     let '(mkBoundedSet cx _) := x in
     let '(mkBoundedSet cy _) := y in
-    mkBoundedSet (AtomSetImpl.inter cx cy) _.
+    mkBoundedSet (set_inter eq_atom_dec cx cy) _.
   Next Obligation.
-    fsetdec.
+    intros a J.
+    apply set_inter_elim in J.
+    destruct J as [J1 J2].
+    eauto.
   Qed.
+
   Lemma lub_commut: forall x y, eq (lub x y) (lub y x).
   Proof.
-    unfold lub, eq. destruct x, y. fsetdec.
+    unfold lub, eq. destruct x, y. 
+    split.
+      intros a J.
+      apply set_inter_elim in J. destruct J.
+      apply set_inter_intro; auto.
+
+      intros a J.
+      apply set_inter_elim in J. destruct J.
+      apply set_inter_intro; auto.
   Qed.
+
   Lemma ge_lub_left: forall x y, ge (lub x y) x.
   Proof.
     unfold lub, ge, sub, eq. destruct x, y. simpl.
-    right. right. fsetdec.
+    right. right.
+    intros a J.
+    apply set_inter_elim in J. destruct J. auto.
   Qed.
 
   Program Definition add (x:t) (a:atom) : t := 
     let '(mkBoundedSet cx _) := x in
-    if (AtomSetProperties.In_dec a bound) then
-      mkBoundedSet (AtomSetImpl.add a cx) _
+    if (In_dec eq_atom_dec a bound) then
+      mkBoundedSet (a::cx) _
     else
       x.
   Next Obligation.
-    assert ({{a}} [<=] bound) as J. 
-      clear - H.
-      admit. (* fsetdec? *)
-    fsetdec.
+    intros a' J.
+    simpl in J.
+    destruct J; subst; eauto.
   Qed.
 
   End VarBoundSec. 
@@ -170,7 +310,7 @@ Module L := Dominators.
 
 Section Kildall.
 
-Variable bound : atoms.
+Variable bound : set atom.
 Definition dt := L.t bound.
 Variable successors: ATree.t (list atom).
 Variable transf: atom -> dt -> dt.
@@ -233,7 +373,7 @@ Definition propagate_succ (s: state) (out: dt) (n: atom) :=
 (** [propagate_succ_list] corresponds, in the pseudocode,
   to the [for] loop iterating over all successors. *)
 
-Fixpoint propagate_succ_list (s: state) (out: dt) (succs: list atom)
+Fixpoint propagate_succ_list (s: state) (out: dt) (succs: set atom)
                              {struct succs} : state :=
   match succs with
   | nil => s
@@ -610,7 +750,7 @@ Fixpoint successors (f: fdef) : ATree.t ls :=
 let '(fdef_intro _ bs) := f in
 successors_blocks bs.
 
-Definition transfer (bound: atoms) (lbl: l) (before: Dominators.t bound) :=
+Definition transfer (bound: set atom) (lbl: l) (before: Dominators.t bound) :=
   Dominators.add _ before lbl.
 
 (** The static analysis itself is then an instantiation of Kildall's
@@ -621,13 +761,13 @@ Definition transfer (bound: atoms) (lbl: l) (before: Dominators.t bound) :=
 
 Module DomDS := Dataflow_Solver_Var_Top(AtomNodeSet).
 
-Fixpoint bound_blocks (bs: blocks) :  atoms :=
+Fixpoint bound_blocks (bs: blocks) : set atom :=
 match bs with
-| nil => {}
-| block_intro l0 _ _ tmn :: bs' => {{l0}} `union` (bound_blocks bs')
+| nil => empty_set _
+| block_intro l0 _ _ tmn :: bs' => l0::(bound_blocks bs')
 end.
 
-Fixpoint bound_fdef (f: fdef) :  atoms :=
+Fixpoint bound_fdef (f: fdef) :  set atom :=
 let '(fdef_intro _ bs) := f in
 bound_blocks bs.
 
@@ -637,7 +777,7 @@ Program Definition dom_analyze (f: fdef): AMap.t (Dominators.t (bound_fdef f)) :
   match getEntryBlock f with
   | Some (block_intro le _ _ _) =>
       match DomDS.fixpoint bound (successors f) (transfer bound) 
-        ((le, Dominators.mkBoundedSet _ {{le}} _) :: nil) with
+        ((le, Dominators.mkBoundedSet _ [le] _) :: nil) with
       | None => AMap.init top
       | Some res => res
       end
@@ -646,7 +786,8 @@ Program Definition dom_analyze (f: fdef): AMap.t (Dominators.t (bound_fdef f)) :
 Next Obligation.
   destruct f. 
   destruct b; simpl in *; inv Heq_anonymous. 
-    fsetdec.
+    simpl_env.
+    apply incl_appl; auto using incl_refl.
 Qed.
 
 Definition blockDominates (f: fdef) (b1 b2: block) : Prop :=
@@ -654,14 +795,14 @@ let '(block_intro l1 _ _ _) := b1 in
 let '(block_intro l2 _ _ _) := b2 in
 let 'dt := dom_analyze f in
 let '(Dominators.mkBoundedSet els _) := AMap.get l2 dt in
-AtomSetProperties.In_dec l1 els.
+In_dec eq_atom_dec l1 els.
 
 Definition blockDominatesB (f: fdef) (b1 b2: block) : Prop :=
 let '(block_intro l1 _ _ _) := b1 in
 let '(block_intro l2 _ _ _) := b2 in
 let 'dt := dom_analyze f in
 let '(Dominators.mkBoundedSet els _) := AMap.get l2 dt in
-if AtomSetProperties.In_dec l1 els then true else false.
+if In_dec eq_atom_dec l1 els then true else false.
 
 Definition insnDominates (i1 i2:insn) (b:block) : Prop :=
 match b with 
