src/ssa/ssa_wf.v
@@ -24,125 +24,110 @@ Require Import Kildall.
 Require Import ssa_analysis.
 Require Import ssa_static.
 Require Import ssa_dynamic.
+Require Import ssa_props.
 
 Export LLVMwf.
+Export AtomSet.
 
-  Definition getCmdID' (i:cmd) : option id :=
-  match i with
-  | insn_bop id _ sz v1 v2 => Some id
-  | insn_fbop id _ _ _ _ => Some id
-  (* | insn_extractelement id typ0 id0 c1 => id *)
-  (* | insn_insertelement id typ0 id0 typ1 v1 c2 => id *)
-  | insn_extractvalue id typs id0 c1 => Some id
-  | insn_insertvalue id typs id0 typ1 v1 c2 => Some id 
-  | insn_malloc id _ _ _ => Some id
-  | insn_free id _ _ => None
-  | insn_alloca id _ _ _ => Some id
-  | insn_load id typ1 v1 _ => Some id
-  | insn_store id typ1 v1 v2 _ => None
-  | insn_gep id _ _ _ _ => Some id
-  | insn_trunc id _ typ1 v1 typ2 => Some id 
-  | insn_ext id _ sz1 v1 sz2 => Some id
-  | insn_cast id _ typ1 v1 typ2 => Some id
-  | insn_icmp id cond typ v1 v2 => Some id
-  | insn_fcmp id cond typ v1 v2 => Some id 
-  | insn_select id v0 typ v1 v2 => Some id
-  | insn_call id nr _ typ v0 paraml => if nr then None else Some id
-  end.
- 
-Fixpoint cmds_dominates_cmd_aux (cs:cmds) (id0:id) (ctx:atoms) : option atoms :=
-match cs with
-| nil => None
-| c1::cs' => 
-    match getCmdID' c1 with
-    | Some id1 =>
-      if eq_atom_dec id1 id0 then 
-        Some ctx 
-      else cmds_dominates_cmd_aux cs' id0 ({{id1}} `union` ctx)
-    | None => Some ctx
-    end
+Definition getCmdID' (i:cmd) : option id :=
+match i with
+| insn_bop id _ sz v1 v2 => Some id
+| insn_fbop id _ _ _ _ => Some id
+(* | insn_extractelement id typ0 id0 c1 => id *)
+(* | insn_insertelement id typ0 id0 typ1 v1 c2 => id *)
+| insn_extractvalue id typs id0 c1 => Some id
+| insn_insertvalue id typs id0 typ1 v1 c2 => Some id 
+| insn_malloc id _ _ _ => Some id
+| insn_free id _ _ => None
+| insn_alloca id _ _ _ => Some id
+| insn_load id typ1 v1 _ => Some id
+| insn_store id typ1 v1 v2 _ => None
+| insn_gep id _ _ _ _ => Some id
+| insn_trunc id _ typ1 v1 typ2 => Some id 
+| insn_ext id _ sz1 v1 sz2 => Some id
+| insn_cast id _ typ1 v1 typ2 => Some id
+| insn_icmp id cond typ v1 v2 => Some id
+| insn_fcmp id cond typ v1 v2 => Some id 
+| insn_select id v0 typ v1 v2 => Some id
+| insn_call id nr _ typ v0 paraml => if nr then None else Some id
 end.
 
-Definition cmds_dominates_cmd (cs:cmds) (id0:id) : option atoms :=
-cmds_dominates_cmd_aux cs id0 {}. 
-
-Fixpoint getCmdsIDs (cs:cmds) : atoms :=
+Fixpoint cmds_dominates_cmd_aux (cs:cmds) (id0:id) (ctx:list atom) : list atom :=
 match cs with
-| nil => {}
+| nil => ctx
+| c1::cs' => 
+    if eq_atom_dec (getCmdID c1) id0 then ctx
+    else
+      match getCmdID' c1 with
+      | Some id1 =>cmds_dominates_cmd_aux cs' id0 (id1::ctx)
+      | None => cmds_dominates_cmd_aux cs' id0 ctx
+      end
+end.
+
+Definition cmds_dominates_cmd (cs:cmds) (id0:id) : list atom :=
+cmds_dominates_cmd_aux cs id0 nil. 
+
+Fixpoint getCmdsIDs' (cs:cmds) : list atom :=
+match cs with
+| nil => nil
 | c::cs' =>
     match getCmdID' c with 
-    | Some id1 => {{id1}} `union` getCmdsIDs cs'
-    | None => getCmdsIDs cs'
+    | Some id1 => id1::getCmdsIDs' cs'
+    | None => getCmdsIDs' cs'
     end
 end.
 
-Fixpoint getPhiNodesIDs' (ps: phinodes) : atoms :=
+Fixpoint getPhiNodesIDs' (ps: phinodes) : list atom :=
 match ps with
-| nil => {}
-| p::ps' => 
-    let id1 := getPhiNodeID p in 
-    {{id1}} `union` getPhiNodesIDs' ps'
+| nil => nil
+| p::ps' => getPhiNodeID p :: getPhiNodesIDs' ps'
 end.
 
-Definition getBlockIDs (b:block) : atoms :=
+Definition getBlockIDs' (b:block) : list atom :=
 let '(block_intro _ ps cs _) := b in
-getPhiNodesIDs' ps `union` getCmdsIDs cs.
+getPhiNodesIDs' ps ++ getCmdsIDs' cs.
 
-Fixpoint getArgsIDs (la:args) : atoms :=
+Fixpoint getArgsIDs' (la:args) : list atom :=
 match la with
-| nil => {}
-| (_,id1)::la' => {{id1}} `union` getArgsIDs la'
+| nil => nil
+| (_,id1)::la' => id1::getArgsIDs' la'
 end.
 
-Definition inscope_of_cmd (f:fdef) (b1:block) (c:cmd) : option atoms :=
+Definition inscope_of_block (f:fdef) (l1:l) (opt_ctx:option (list atom)) (lbl:l)
+  :=
+  match opt_ctx with
+  | Some ctx =>
+     match lookupBlockViaIDFromFdef f lbl with
+     | None => None
+     | Some b => 
+         if eq_atom_dec lbl l1 then Some ctx
+         else Some (getBlockIDs' b ++ ctx)
+     end
+  | None => None
+  end.
+
+Definition inscope_of_cmd (f:fdef) (b1:block) (c:cmd) : option (list atom) :=
 let id0 := getCmdID c in
 let '(block_intro l1 ps cs _) := b1 in
 let '(fdef_intro (fheader_intro _ _ la) _) := f in
 let 'dt := dom_analyze f in
 let '(Dominators.mkBoundedSet els _) := AMap.get l1 dt in
-match cmds_dominates_cmd cs id0 with
-| None => None
-| Some ids' => 
-    fold_left 
-      (fun (opt_ctx:option atoms) (lbl:l) =>
-         match opt_ctx with
-         | Some ctx =>
-           match lookupBlockViaIDFromFdef f lbl with
-           | None => None
-           | Some b => 
-               if eq_atom_dec lbl l1 then Some ctx
-               else Some (getBlockIDs b `union` ctx)
-           end
-         | None => None
-         end
-      )
-      (AtomSetImpl.elements els) 
-      (Some (getPhiNodesIDs' ps `union` ids' `union` getArgsIDs la))
-end.
+fold_left (inscope_of_block f l1) els
+  (Some (getPhiNodesIDs' ps ++ cmds_dominates_cmd cs id0 ++ getArgsIDs' la))
+.
 
-Definition inscope_of_tmn (f:fdef) (b1:block) (tmn:terminator) : option atoms :=
+Definition inscope_of_tmn (f:fdef) (b1:block) (tmn:terminator) 
+  : option (list atom) :=
 let '(block_intro l1 ps cs _) := b1 in
 let '(fdef_intro (fheader_intro _ _ la) _) := f in
 let 'dt := dom_analyze f in
 let '(Dominators.mkBoundedSet els _) := AMap.get l1 dt in
-fold_left 
-  (fun (opt_ctx:option atoms) (lbl:l) =>
-     match opt_ctx with
-     | Some ctx =>
-       match lookupBlockViaIDFromFdef f lbl with
-       | None => None
-       | Some b => 
-         if eq_atom_dec lbl l1 then Some ctx
-         else Some (getBlockIDs b `union` ctx)
-       end
-     | None => None
-     end
-  )
-  (AtomSetImpl.elements els) 
-  (Some (getPhiNodesIDs' ps `union` getCmdsIDs cs `union` getArgsIDs la)).
+fold_left (inscope_of_block f l1) els
+  (Some (getPhiNodesIDs' ps ++ getCmdsIDs' cs ++ getArgsIDs' la))
+.
 
-Definition defs_dominate (f:fdef) (curb incomingb:block) (i:insn) : option atoms 
-  :=
+Definition defs_dominate (f:fdef) (curb incomingb:block) (i:insn) 
+  : option (list atom) :=
 match i with
 | insn_phinode p => 
     let '(block_intro _ _ _ tmn) := incomingb in
@@ -158,29 +143,85 @@ Export LLVMopsem.
 Inductive wf_genericvalue : GenericValue -> typ -> Prop :=
 | wf_genericvalue_intro : forall gv t, wf_genericvalue gv t.
 
-Inductive wf_defs : fdef -> GVMap -> ids -> Prop :=
-| wf_defs_nil : forall f lc, wf_defs f lc nil
-| wf_defs_cons : forall f lc id1 gv1 t1 ids',
+Inductive wf_defs (f:fdef) (lc:GVMap) : list atom -> Prop :=
+| wf_defs_nil : wf_defs f lc nil
+| wf_defs_cons : forall id1 t1 gv1 defs',
     lookupTypViaIDFromFdef f id1 = Some t1 ->
+    lookupAL _ lc id1 = Some gv1 ->
     wf_genericvalue gv1 t1 ->
-    wf_defs f lc ids' ->
-    wf_defs f lc (id1::ids')
-.
+    wf_defs f lc defs' ->
+    wf_defs f lc (id1::defs').
+
+Lemma wf_defs__forall : forall ids1 F lc,
+  wf_defs F lc ids1 ->
+  forall id1, In id1 ids1 ->
+  exists t1, exists gv1,
+    lookupTypViaIDFromFdef F id1 = Some t1 /\
+    lookupAL _ lc id1 = Some gv1 /\
+    wf_genericvalue gv1 t1.
+Proof.
+  induction ids1; intros; simpl in H0; inv H0.  
+    inv H.
+    exists t1. exists gv1. split; auto.
+
+    inv H.
+    eapply IHids1 in H6; eauto.
+Qed.    
+
+Lemma forall__wf_defs : forall ids1 F lc,
+  (forall id1, In id1 ids1 ->
+   exists t1, exists gv1,
+     lookupTypViaIDFromFdef F id1 = Some t1 /\
+     lookupAL _ lc id1 = Some gv1 /\
+     wf_genericvalue gv1 t1) ->
+  wf_defs F lc ids1.
+Proof.
+  induction ids1; intros.
+    apply wf_defs_nil.  
+
+    destruct (@H a) as [t1 [gv1 [J1 [J2 J3]]]]; simpl; auto.
+    eapply wf_defs_cons; eauto.
+      apply IHids1.
+      intros id1 J.
+      apply H. simpl. auto.
+Qed.
+
+Lemma wf_defs_eq : forall ids2 ids1 F' lc',
+  set_eq _ ids1 ids2 ->
+  wf_defs F' lc' ids1 ->
+  wf_defs F' lc' ids2.
+Proof.
+  intros.
+  apply forall__wf_defs.
+  intros id1 Hin.
+  destruct H as [J1 J2].
+  eapply wf_defs__forall in H0; eauto.
+Qed.
+
+Lemma wf_defs_updateAddAL : forall g TD Mem' Result lc gl F' lc' ids1 ids2 i1,
+  ret g = getOperandValue TD Mem' Result lc gl ->
+  wf_defs F' lc' ids1 ->
+  set_eq _ (i1::ids1) ids2 ->
+  wf_defs F' (updateAddAL GenericValue lc' i1 g) ids2.
+Proof.
+  intros g TD Mem' Result lc gl F' lc' ids1 ids2 i1 Hget HwfDefs Heq.
+  (* need to show that g is welltyped.*)
+Admitted.
 
 Definition wf_ExecutionContext (ps:list product) (ec:ExecutionContext) : Prop :=
 let '(mkEC f b cs tmn lc als) := ec in
-(*isReachableFromEntry f b /\*)
+isReachableFromEntry f b /\
 blockInFdefB b f = true /\
 InProductsB (product_fdef f) ps = true /\
 match cs with
 | nil => 
     match inscope_of_tmn f b tmn with
-    | Some ids => wf_defs f lc (AtomSetImpl.elements ids)
+    | Some ids => wf_defs f lc ids
     | None => False
     end
 | c::_ =>
     match inscope_of_cmd f b c with
-    | Some ids => wf_defs f lc (AtomSetImpl.elements ids)
+    | Some ids => wf_defs f lc ids
     | None => False
     end
 end /\
@@ -188,7 +229,9 @@ exists l1, exists ps, exists cs',
 b = block_intro l1 ps (cs'++cs) tmn.
 
 Definition wf_call (ec:ExecutionContext) (ecs:ECStack) : Prop :=
-let '(mkEC f b cs tmn lc als) := ec in
+let '(mkEC f _ _ _ _ _) := ec in
+forall b, blockInFdefB b f ->
+let '(block_intro _ _ _ tmn) := b in
 match tmn with
 | insn_return _ _ _ =>
     match ecs with
@@ -217,43 +260,552 @@ wf_system nil s /\
 moduleInSystemB (module_intro los nts ps) s = true /\
 wf_ECStack ps ecs.
 
+Lemma getCmdID_getCmdID' : forall a i0,
+  getCmdID' a = Some i0 ->
+  getCmdID a = i0.
+Proof.
+  intros a i0 H.
+  destruct a; inv H; auto.
+    simpl. destruct n; inv H1; auto.
+Qed.
+
+Lemma set_eq_app : forall x1 x2 y1 y2,
+  set_eq atom x1 y1 -> set_eq atom x2 y2 -> set_eq atom (x1++x2) (y1++y2).
+Admitted.
+
+Lemma set_eq_swap : forall x1 x2,
+  set_eq atom (x1++x2) (x2++x1).
+Admitted.
+
+Lemma set_eq_empty_inv2 : forall x, 
+  set_eq atom (ListSet.empty_set _) x -> x = ListSet.empty_set _.
+Proof.
+  intros.
+  apply set_eq_sym in H.
+  eapply set_eq_empty_inv; eauto.
+Qed.
+
+Lemma cmds_dominates_cmd_aux__eq : forall cs id0 defs1 defs2,
+  set_eq _ defs1 defs2 ->
+  set_eq _ (cmds_dominates_cmd_aux cs id0 defs1)
+           (cmds_dominates_cmd_aux cs id0 defs2).
+Proof.
+  induction cs; intros id0 defs1 defs2 Heq; simpl; auto.
+    destruct (eq_atom_dec (getCmdID a) id0); auto.
+    destruct (getCmdID' a); auto.
+Admitted.
+
+Lemma cmds_dominates_cmd_aux__commut : forall cs id0 defs1 defs2,
+  set_eq _ (cmds_dominates_cmd_aux cs id0 (defs1 ++ defs2))
+           (defs1 ++ cmds_dominates_cmd_aux cs id0 defs2).
+Proof.
+  induction cs; intros; simpl.
+    apply set_eq_refl.
+
+    remember (getCmdID a) as id1.
+    destruct (eq_atom_dec id1 id0); subst.
+      apply set_eq_refl.
+
+      remember (getCmdID' a) as R.
+      destruct R; auto.
+        eapply set_eq_trans with 
+          (y:=cmds_dominates_cmd_aux cs id0 (defs1 ++ i0 :: defs2)); eauto.
+        apply cmds_dominates_cmd_aux__eq.
+          rewrite_env (([i0]++defs1)++defs2).
+          rewrite_env ((defs1++[i0])++defs2).
+          apply set_eq_app.
+             apply set_eq_swap; auto.
+             apply set_eq_refl.
+Qed.
+
+Lemma getCmdsIDs__cmds_dominates_cmd : forall cs2' c',
+  ~ In (getCmdID c') (LLVMlib.getCmdsIDs cs2') ->
+  set_eq _ (getCmdsIDs' (cs2' ++ [c']))
+  (cmds_dominates_cmd (cs2' ++ [c']) (getCmdID c') ++ 
+    match getCmdID' c' with
+    | Some id1 => [id1]
+    | None => nil
+    end).   
+Proof.
+  unfold cmds_dominates_cmd.
+  induction cs2'; intros c' Hnotin.
+    simpl in *.
+    destruct (eq_atom_dec (getCmdID c') (getCmdID c')) as [_ | n];
+      try solve [contradict n; auto].
+      remember (getCmdID' c') as R.
+      destruct R; simpl_env; apply set_eq_refl.
+
+    simpl in *.
+    assert (~ In (getCmdID c') (getCmdsIDs cs2')) as J.
+      auto.
+    apply IHcs2' in J.
+    remember (getCmdID' a) as R1.
+    remember (getCmdID' c') as R2.
+    destruct (eq_atom_dec (getCmdID a) (getCmdID c')); 
+      try solve [contradict e; auto].
+    destruct R1; auto.
+      simpl_env.
+      apply set_eq_trans with (y:=[i0] ++
+        cmds_dominates_cmd_aux (cs2' ++ [c']) (getCmdID c') nil ++
+        match R2 with
+        | ret id1 => [id1]
+        | merror => nil
+        end).
+        apply set_eq_app; auto using set_eq_refl.
+
+        rewrite_env (([i0] ++
+          cmds_dominates_cmd_aux (cs2' ++ [c']) (getCmdID c') nil) ++
+          match R2 with
+          | ret id1 => [id1]
+          | merror => nil
+          end).
+        apply set_eq_app.
+          apply set_eq_sym.
+          rewrite_env ([i0]++nil).
+          apply cmds_dominates_cmd_aux__commut.
+          apply set_eq_refl.
+Qed.      
+
+Definition opt_set_eq (ops1 ops2:option (list atom)) : Prop :=
+match (ops1, ops2) with
+| (None, None) => True
+| (Some s1, Some s2) => set_eq _ s1 s2
+| _ => False
+end.
+
+Lemma inscope_of_block__opt_set_eq : forall f l1 l' opr1 opr2,
+  opt_set_eq opr1 opr2 ->
+  opt_set_eq (inscope_of_block f l1 opr1 l') (inscope_of_block f l1 opr2 l').
+Proof.
+  unfold inscope_of_block.
+  intros.
+  destruct (lookupBlockViaIDFromFdef f l').
+    destruct (eq_atom_dec l' l1); subst.
+      destruct opr1.
+        destruct opr2; try solve [inversion H | auto].
+        destruct opr2; try solve [inversion H | auto].
+      unfold opt_set_eq in *.
+      destruct opr1.
+        destruct opr2; try solve [inversion H ].
+          apply set_eq_app; auto using set_eq_refl.
+        destruct opr2; try solve [inversion H | auto ].
+    unfold opt_set_eq in *.
+    destruct opr1.
+      destruct opr2; try solve [inversion H | auto].
+      destruct opr2; try solve [inversion H | auto].
+Qed.
+ 
+Lemma fold_left__opt_set_eq_aux : forall ls0 opr1 opr2 f l1,
+  opt_set_eq opr1 opr2 ->
+  opt_set_eq (fold_left (inscope_of_block f l1) ls0 opr1) 
+           (fold_left (inscope_of_block f l1) ls0 opr2).
+Proof.
+  induction ls0; intros opr1 opr2 f l1 Heq; simpl in *; auto.
+    apply IHls0.
+      apply inscope_of_block__opt_set_eq; auto.
+Qed.
+
+Lemma fold_left__opt_set_eq : forall (ls0:list atom) f l1 init1 init2 r1,
+  set_eq _ init1 init2 ->  
+  fold_left (inscope_of_block f l1) ls0 (Some init1) = Some r1 ->
+  exists r2, fold_left (inscope_of_block f l1) ls0 (Some init2) = Some r2 /\ 
+    set_eq _ r1 r2.
+Proof.
+  intros.
+  assert (opt_set_eq (Some init1) (Some init2)) as EQ. unfold opt_set_eq. auto.
+  apply fold_left__opt_set_eq_aux with (ls0:=ls0)(f:=f)(l1:=l1) in EQ.
+  remember (fold_left (inscope_of_block f l1) ls0 (ret init2)) as R. 
+  unfold opt_set_eq in EQ.    
+  rewrite H0 in EQ.
+  destruct R; try solve [inversion EQ].
+  exists l0. auto.
+Qed.
+ 
+Lemma inscope_of_block__opt_union : forall f l1 l' init1 init2 r1,
+  inscope_of_block f l1 (Some init1) l' = Some r1 ->
+  exists r2, inscope_of_block f l1 (Some (init1++init2)) l' = Some r2 /\
+    set_eq _ (r1++init2) r2.
+Proof.
+  intros.
+  unfold inscope_of_block in *.
+  destruct (lookupBlockViaIDFromFdef f l').
+    destruct (eq_atom_dec l' l1); subst; inv H.
+      exists (r1++init2). auto using set_eq_refl.
+      exists (getBlockIDs' b ++ init1 ++ init2). 
+        simpl_env. auto using set_eq_refl.
+    inversion H.
+Qed.
+
+Lemma fold_left__none : forall (ls0:list atom) f l1,
+  fold_left (inscope_of_block f l1) ls0 None = None.
+Proof.
+  induction ls0; intros f l1; simpl in *; auto.
+Qed.
+
+Lemma fold_left__opt_union : forall (ls0:list atom) f l1 init1 init2 r1,
+  fold_left (inscope_of_block f l1) ls0 (Some init1) = Some r1 ->
+  exists r2, 
+    fold_left (inscope_of_block f l1) ls0 (Some (init1++init2)) = Some r2 
+      /\ set_eq _ (r1++init2) r2.
+Proof.
+  induction ls0; intros f l1 init1 init2 r1 H; simpl in *; auto.
+    inv H. exists (r1 ++ init2). split; auto using set_eq_refl.
+
+    destruct (lookupBlockViaIDFromFdef f a).
+      destruct (eq_atom_dec a l1); subst; auto.
+        apply IHls0 with (init2:=init2) in H; auto.
+          simpl_env in H. auto.
+      rewrite fold_left__none in H. inversion H.
+Qed.
+
 Lemma inscope_of_cmd_tmn : forall f l2 ps2 cs2' c' tmn' ids1,
+~ In (getCmdID c') (getCmdsIDs cs2') ->
 Some ids1 = inscope_of_cmd f (block_intro l2 ps2 (cs2'++[c']) tmn') c' ->
 exists ids2, 
   Some ids2 = inscope_of_tmn f (block_intro l2 ps2 (cs2'++[c']) tmn') tmn' /\
   match getCmdID' c' with
-  | Some id1 => {{id1}} `union` ids1 [=] ids2
-  | None => ids1 [=] ids2
+  | Some id1 => set_eq _ (id1::ids1) ids2
+  | None => set_eq _ ids1 ids2
   end.
-Admitted.
+Proof.
+  intros f l2 ps2 cs2' c' tmn' ids1 Hnotin Hinscope.
+  unfold inscope_of_cmd in Hinscope.
+  unfold inscope_of_tmn.
+  destruct f as [[? ? la] bs].
+  remember ((dom_analyze (fdef_intro (fheader_intro t i0 la) bs)) !! l2) as R.
+  destruct R as [R_contents R_bound]. simpl in *.
+  apply getCmdsIDs__cmds_dominates_cmd in Hnotin.
+  symmetry in Hinscope.
+  remember (getCmdID' c') as R.
+  destruct R.
+    apply fold_left__opt_union with (init2:=[i1]) in Hinscope.
+    destruct Hinscope as [r2 [Hinscope Heq]].
+    apply fold_left__opt_set_eq with (init2:=((getPhiNodesIDs' ps2) ++
+      ((getCmdsIDs' (cs2' ++ [c'])) ++ (getArgsIDs' la)))) in Hinscope.
+      destruct Hinscope as [r3 [Hinscope Heq']].
+      exists r3.     
+      split; auto.
+        simpl_env. 
+        eapply set_eq_trans with (y:=r2); eauto.
+        eapply set_eq_trans with (y:=ids1 ++ [i1]); eauto.
+          apply set_eq_swap.          
+      simpl_env.
+      apply set_eq_app; auto using set_eq_refl.
+      apply set_eq_trans with (y:=(cmds_dominates_cmd (cs2' ++ [c']) 
+         (getCmdID c') ++ [i1]) ++ getArgsIDs' la).
+        simpl_env.
+        apply set_eq_app; auto using set_eq_refl.
+          apply set_eq_swap.          
 
-Lemma wf_defs_updateAddAL : forall g TD Mem' Result lc gl F' lc' t ids2 i1,
-  ret g = getOperandValue TD Mem' Result lc gl ->
-  wf_defs F' lc' (AtomSetImpl.elements t) ->
-  union (singleton i1) t[=]ids2 ->
-  wf_defs F' (updateAddAL GenericValue lc' i1 g) (AtomSetImpl.elements ids2).
-Admitted.
+        apply set_eq_app; auto using set_eq_refl.
+          apply set_eq_sym; auto.          
 
-Lemma wf_defs_eq : forall ids1 ids2 F' lc',
-  ids1 [=] ids2 ->
-  wf_defs F' lc' (AtomSetImpl.elements ids1) ->
-  wf_defs F' lc' (AtomSetImpl.elements ids2).
-Admitted.
+    apply fold_left__opt_set_eq with (init2:=((getPhiNodesIDs' ps2) ++ 
+      ((getCmdsIDs' (cs2' ++ [c'])) ++ (getArgsIDs' la)))) in Hinscope.
+      destruct Hinscope as [r3 [Hinscope Heq']].
+      exists r3.     
+      split; auto.
+      apply set_eq_app; auto using set_eq_refl.
+      apply set_eq_app; auto using set_eq_refl.
+      simpl_env in Hnotin.
+      apply set_eq_sym; auto.          
+Qed.
+
+Lemma set_eq__rewrite_env : forall x1 x2 x3 y1 y2 y3,
+  set_eq atom ((x1 ++ x2) ++ x3) ((y1 ++ y2) ++ y3) ->
+  set_eq atom (x1 ++ x2 ++ x3) (y1 ++ y2 ++ y3).
+Proof.
+  intros.
+  simpl_env in H. auto.
+Qed.
+
+Lemma cmds_dominates_cmd__cmds_dominates_cmd : forall cs2' c' c cs',
+  NoDup (getCmdsIDs (cs2'++[c']++[c]++cs')) ->
+  set_eq _ (cmds_dominates_cmd (cs2' ++ c' :: c :: cs') (getCmdID c))
+    (cmds_dominates_cmd (cs2' ++ c' :: c :: cs') (getCmdID c') ++
+     match getCmdID' c' with
+     | Some id1 => [id1]
+     | None => nil
+     end).   
+Proof.
+  unfold cmds_dominates_cmd in *.
+  induction cs2'; intros c' c cs' Hnodup.
+    simpl in *.
+    inv Hnodup. simpl in H1.
+    remember (getCmdID' c') as R.
+    destruct (eq_atom_dec (getCmdID c') (getCmdID c)).
+      contradict e; auto.
+
+      destruct (eq_atom_dec (getCmdID c) (getCmdID c)) as [_|n1];
+        try solve [contradict n1; auto].
+      destruct (eq_atom_dec (getCmdID c') (getCmdID c')) as [_|n2];
+        try solve [contradict n2; auto].
+      destruct R; auto using set_eq_refl.
+
+    simpl in *.
+    inv Hnodup.
+    rewrite getCmdsIDs_app in H1.
+    apply NotIn_inv in H1.    
+    destruct H1 as [H11 H12].
+    simpl in H12.
+    destruct (eq_atom_dec (getCmdID a) (getCmdID c)) as [e1 | ];
+      try solve [contradict e1; auto].
+    destruct (eq_atom_dec (getCmdID a) (getCmdID c')) as [e1 | ];
+      try solve [contradict e1; auto].
+    destruct (getCmdID' a); auto.
+      apply IHcs2' in H2. clear IHcs2'.
+      rewrite_env ([i0]++nil).
+      apply set_eq_trans with (y:=[i0]++
+        (cmds_dominates_cmd_aux (cs2' ++ c' :: c :: cs') (getCmdID c) nil)).
+        apply cmds_dominates_cmd_aux__commut.
+      apply set_eq_trans with (y:=[i0] ++
+        (cmds_dominates_cmd_aux (cs2' ++ c' :: c :: cs') (getCmdID c') nil ++
+         match getCmdID' c' with
+         | ret id1 => [id1]
+         | merror => nil
+         end)).
+       apply set_eq_app; auto using set_eq_refl.
+
+       rewrite_env (([i0] ++
+         cmds_dominates_cmd_aux (cs2' ++ c' :: c :: cs') (getCmdID c') nil) ++
+         match getCmdID' c' with
+         | ret id1 => [id1]
+         | merror => nil
+         end).
+       apply set_eq_app; auto using set_eq_refl.
+       apply set_eq_sym.
+         apply cmds_dominates_cmd_aux__commut.
+Qed.      
 
 Lemma inscope_of_cmd_cmd : forall f l2 ps2 cs2' c' c cs' tmn' ids1,
+NoDup (getCmdsIDs (cs2'++[c']++[c]++cs')) ->
 Some ids1 = inscope_of_cmd f (block_intro l2 ps2 (cs2'++[c']++[c]++cs') tmn') c' 
   ->
 exists ids2, 
   Some ids2 = 
     inscope_of_cmd f (block_intro l2 ps2 (cs2'++[c']++[c]++cs') tmn') c /\
   match getCmdID' c' with
-  | Some id1 => {{id1}} `union` ids1 [=] ids2
-  | None => ids1 [=] ids2
+  | Some id1 => set_eq _ (id1::ids1) ids2
+  | None => set_eq _ ids1 ids2
   end.
+Proof.
+  intros f l2 ps2 cs2' c' c cs' tmn' ids1 Hnodup Hinscope.
+  unfold inscope_of_cmd in Hinscope.
+  unfold inscope_of_cmd.
+  destruct f as [[? ? la] bs].
+  remember ((dom_analyze (fdef_intro (fheader_intro t i0 la) bs)) !! l2) as R.
+  destruct R as [R_contents R_bound].
+  apply cmds_dominates_cmd__cmds_dominates_cmd in Hnodup. simpl in *.
+  symmetry in Hinscope.
+  remember (getCmdID' c') as R.
+  destruct R.
+    apply fold_left__opt_union with (init2:=[i1]) in Hinscope.
+    destruct Hinscope as [r2 [Hinscope Heq]].
+    apply fold_left__opt_set_eq with (init2:=((getPhiNodesIDs' ps2) ++ 
+      ((cmds_dominates_cmd (cs2' ++ c' :: c :: cs') (getCmdID c)) ++
+      (getArgsIDs' la)))) in Hinscope.
+      destruct Hinscope as [r3 [Hinscope Heq']].
+      exists r3.     
+      split; auto.
+        simpl_env. 
+        eapply set_eq_trans with (y:=r2); eauto.
+        eapply set_eq_trans with (y:=ids1 ++ [i1]); eauto.
+          apply set_eq_swap.          
+      simpl_env.
+      apply set_eq_app; auto using set_eq_refl.
+      apply set_eq_trans with (y:=(cmds_dominates_cmd (cs2' ++ [c']++[c]++cs') 
+         (getCmdID c') ++ [i1]) ++ getArgsIDs' la).
+        simpl_env.
+        apply set_eq_app; auto using set_eq_refl.
+          apply set_eq_swap.          
+
+        apply set_eq_app; auto using set_eq_refl.
+          apply set_eq_sym; auto.          
+
+    apply fold_left__opt_set_eq with (init2:=((getPhiNodesIDs' ps2) ++
+      ((cmds_dominates_cmd (cs2' ++ c' :: c :: cs') (getCmdID c)) ++
+      (getArgsIDs' la)))) in Hinscope.
+      destruct Hinscope as [r3 [Hinscope Heq']].
+      exists r3.     
+      split; auto.
+      apply set_eq_app; auto using set_eq_refl.
+      apply set_eq_app; auto using set_eq_refl.
+      simpl_env in Hnodup.
+      apply set_eq_sym; auto.          
+Qed.
+
+Lemma fold_left__bound_blocks : forall ls0 t i0 la bs l0 init,
+  incl ls0 (bound_blocks bs) ->
+  exists r, 
+    fold_left (inscope_of_block 
+                (fdef_intro (fheader_intro t i0 la) bs) l0) ls0 (Some init) = 
+      Some r.
 Admitted.
+
+Lemma fold_left__spec : forall ls0 l0 init r f,
+  fold_left (inscope_of_block f l0) ls0 (Some init) = Some r ->
+    incl init r /\
+    (forall l1 b1, 
+      In l1 ls0 -> l1 <> l0 -> 
+      lookupBlockViaIDFromFdef f l1 = Some b1 ->
+      incl (getBlockIDs' b1) r) /\
+    (forall id1,
+      In id1 r ->
+      In id1 init \/
+      exists b1, exists l1, l1 <> l0 /\ In l1 ls0 /\
+        lookupBlockViaIDFromFdef f l1 = Some b1 /\
+        In id1 (getBlockIDs' b1)
+    ).
+Admitted.
+
+Lemma fold_left__incl : forall ls0 f l0 init ls1 r0 r1,
+  incl ls0 ls1 ->
+  fold_left (inscope_of_block f l0) ls0 (Some init) = Some r0 ->
+  fold_left (inscope_of_block f l0) ls1 (Some init) = Some r1 ->
+  incl r0 r1.
+Admitted.
+
+Lemma inscope_of_tmn_br_aux : forall F l3 ps cs tmn ids0 l' ps' cs' tmn' l0,
+uniqFdef F ->
+blockInFdefB (block_intro l3 ps cs tmn) F = true ->
+In l0 (successors_terminator tmn) ->
+Some ids0 = inscope_of_tmn F (block_intro l3 ps cs tmn) tmn ->
+Some (block_intro l' ps' cs' tmn') = lookupBlockViaLabelFromFdef F l0 ->
+exists ids0',
+  match cs' with
+  | nil => Some ids0' = inscope_of_tmn F (block_intro l' ps' cs' tmn') tmn'
+  | c'::_ => Some ids0' = inscope_of_cmd F (block_intro l' ps' cs' tmn') c'
+  end /\
+  incl (ListSet.set_diff eq_atom_dec ids0' (getPhiNodesIDs' ps')) ids0.
+Proof.
+  intros F l3 ps cs tmn ids0 l' ps' cs' tmn' l0 Huniq HBinF Hsucc Hinscope Hlkup.
+  symmetry in Hlkup.
+  assert (J:=Hlkup).
+  apply lookupBlockViaLabelFromFdef_inv in J; auto.
+  destruct J as [Heq J]; subst.
+  unfold inscope_of_tmn in Hinscope.
+  unfold inscope_of_tmn. unfold inscope_of_cmd.
+  destruct F as [[? ? la] bs].
+  remember ((dom_analyze (fdef_intro (fheader_intro t i0 la) bs)) !! l3)as defs3.
+  remember ((dom_analyze (fdef_intro (fheader_intro t i0 la) bs)) !! l')as defs'.
+  destruct defs3 as [contents3 inbound3]. 
+  destruct defs' as [contents' inbound']. 
+  simpl in *.
+  assert (incl contents' contents3) as Hsub.
+
+
+    admit. (* by correctness of domination analysis *)
+  destruct cs'.
+  Case "cs'=nil".
+    assert (J1:=inbound').
+    apply fold_left__bound_blocks with (init:=getPhiNodesIDs' ps' ++ 
+      getCmdsIDs' nil ++ getArgsIDs' la)(t:=t)(i0:=i0)(la:=la)(bs:=bs)(l0:=l')
+      in J1.
+    destruct J1 as [r J1].
+    exists r. split; auto.
+    clear - Hinscope J1 Hsub HBinF.
+    apply fold_left__spec in J1.
+    symmetry in Hinscope.
+    apply fold_left__spec in Hinscope.
+    destruct J1 as [J1 [J2 J3]].
+    destruct Hinscope as [J4 [J5 J6]].
+    intros id1 J.
+    assert (J':=J).
+    apply ListSet.set_diff_elim1 in J.
+    apply ListSet.set_diff_elim2 in J'.
+    apply J3 in J.
+    destruct J as [J | J].
+    SCase "id1 in init and the current block".
+      simpl in J.
+      apply in_app_or in J.
+      destruct J as [J | J]; try solve [contradict J; auto].
+      apply J4.
+      apply in_or_app. right.
+      apply in_or_app; auto.
+    SCase "id1 in strict dominating blocks".
+      destruct J as [b1 [l1 [J7 [J8 [J9 J10]]]]].
+      apply Hsub in J8.
+        destruct (eq_atom_dec l1 l3); subst.
+          simpl in J9. 
+          assert (b1=block_intro l3 ps cs tmn) as EQ.
+            clear - J9 HBinF. admit.
+          subst.
+          simpl in J10.
+          apply J4.
+          rewrite_env 
+            ((getPhiNodesIDs' ps ++ getCmdsIDs' cs) ++ getArgsIDs' la).
+          apply in_or_app; auto.
+
+          apply J5 in J9; auto.
+          
+  Case "cs'<>nil".
+    assert (J1:=inbound').
+    unfold cmds_dominates_cmd. simpl.
+    destruct (eq_atom_dec (getCmdID c) (getCmdID c)) as [_ | n]; 
+      try solve [contradict n; auto].
+    simpl_env.
+    apply fold_left__bound_blocks with (init:=getPhiNodesIDs' ps' ++ 
+      getArgsIDs' la)(t:=t)(i0:=i0)(la:=la)(bs:=bs)(l0:=l') in J1.
+    destruct J1 as [r J1].
+    exists r. split; auto.
+    clear - Hinscope J1 Hsub HBinF.
+    apply fold_left__spec in J1.
+    symmetry in Hinscope.
+    apply fold_left__spec in Hinscope.
+    destruct J1 as [J1 [J2 J3]].
+    destruct Hinscope as [J4 [J5 J6]].
+    intros id1 J.
+    assert (J':=J).
+    apply ListSet.set_diff_elim1 in J.
+    apply ListSet.set_diff_elim2 in J'.
+    apply J3 in J.
+    destruct J as [J | J].
+    SCase "id1 in init and the current block".
+      simpl in J.
+      apply in_app_or in J.
+      destruct J as [J | J]; try solve [contradict J; auto].
+      apply J4.
+      apply in_or_app. right.
+      apply in_or_app; auto.
+    SCase "id1 in strict dominating blocks".
+      destruct J as [b1 [l1 [J7 [J8 [J9 J10]]]]].
+      apply Hsub in J8.
+        destruct (eq_atom_dec l1 l3); subst.
+          simpl in J9. 
+          assert (b1=block_intro l3 ps cs tmn) as EQ.
+            clear - J9 HBinF. admit.
+          subst.
+          simpl in J10.
+          apply J4.
+          rewrite_env 
+            ((getPhiNodesIDs' ps ++ getCmdsIDs' cs) ++ getArgsIDs' la).
+          apply in_or_app; auto.
+
+          apply J5 in J9; auto. 
+Qed.
+
+Lemma inscope_of_tmn_br_uncond : forall F l3 ps cs bid ids0 l' ps' cs' tmn' l0,
+uniqFdef F ->
+blockInFdefB (block_intro l3 ps cs (insn_br_uncond bid l0)) F = true ->
+Some ids0 = inscope_of_tmn F (block_intro l3 ps cs (insn_br_uncond bid l0)) 
+  (insn_br_uncond bid l0) ->
+Some (block_intro l' ps' cs' tmn') = lookupBlockViaLabelFromFdef F l0 ->
+exists ids0',
+  match cs' with
+  | nil => Some ids0' = inscope_of_tmn F (block_intro l' ps' cs' tmn') tmn'
+  | c'::_ => Some ids0' = inscope_of_cmd F (block_intro l' ps' cs' tmn') c'
+  end /\
+  incl (ListSet.set_diff eq_atom_dec ids0' (getPhiNodesIDs' ps')) ids0.
+Proof.
+  intros.
+  eapply inscope_of_tmn_br_aux; eauto.
+  simpl. auto.
+Qed.
 
 Lemma inscope_of_tmn_br : forall F l0 ps cs bid l1 l2 ids0 l' ps' cs' tmn' Cond 
   c TD Mem0 gl lc,
+uniqFdef F ->
+blockInFdefB (block_intro l0 ps cs (insn_br bid Cond l1 l2)) F = true ->
 Some ids0 = inscope_of_tmn F (block_intro l0 ps cs (insn_br bid Cond l1 l2)) 
   (insn_br bid Cond l1 l2) ->
 getOperandValue TD Mem0 Cond lc gl = ret c ->
@@ -266,8 +818,12 @@ exists ids0',
   | nil => Some ids0' = inscope_of_tmn F (block_intro l' ps' cs' tmn') tmn'
   | c'::_ => Some ids0' = inscope_of_cmd F (block_intro l' ps' cs' tmn') c'
   end /\
-  AtomSetImpl.diff ids0' (getPhiNodesIDs' ps') [<=] ids0.
-Admitted.
+  incl (ListSet.set_diff eq_atom_dec ids0' (getPhiNodesIDs' ps')) ids0.
+Proof.
+  intros.
+  remember (isGVZero TD c) as R.
+  destruct R; eapply inscope_of_tmn_br_aux; eauto; simpl; auto.
+Qed.
 
 Lemma wf_defs_br : forall TD Mem0 Cond lc gl c l' ps' cs' lc' F l1 l2 bid tmn'
   (H : getOperandValue TD Mem0 Cond lc gl = ret c)
@@ -281,23 +837,11 @@ Lemma wf_defs_br : forall TD Mem0 Cond lc gl c l' ps' cs' lc' F l1 l2 bid tmn'
   (H1 : switchToNewBasicBlock TD Mem0 (block_intro l' ps' cs' tmn')
          (block_intro l3 ps3 (cs3' ++ nil) (insn_br bid Cond l1 l2)) gl lc =
        ret lc')
-  (t : atoms)
-  (Hinscope1 : wf_defs F lc (AtomSetImpl.elements t))
-  (ids0' : atoms)
-  (HeqR12 : AtomSetImpl.diff ids0' (getPhiNodesIDs' ps')[<=]t),
-  wf_defs F lc' (AtomSetImpl.elements ids0').
-Admitted.
-
-Lemma inscope_of_tmn_br_uncond : forall F l3 ps cs bid ids0 l' ps' cs' tmn' l0,
-Some ids0 = inscope_of_tmn F (block_intro l3 ps cs (insn_br_uncond bid l0)) 
-  (insn_br_uncond bid l0) ->
-Some (block_intro l' ps' cs' tmn') = lookupBlockViaLabelFromFdef F l0 ->
-exists ids0',
-  match cs' with
-  | nil => Some ids0' = inscope_of_tmn F (block_intro l' ps' cs' tmn') tmn'
-  | c'::_ => Some ids0' = inscope_of_cmd F (block_intro l' ps' cs' tmn') c'
-  end /\
-  AtomSetImpl.diff ids0' (getPhiNodesIDs' ps') [<=] ids0.
+  (t : list atom)
+  (Hinscope1 : wf_defs F lc t)
+  (ids0' : list atom)
+  (HeqR12 : incl (ListSet.set_diff eq_atom_dec ids0' (getPhiNodesIDs' ps')) t),
+  wf_defs F lc' ids0'.
 Admitted.
 
 Lemma wf_defs_br_uncond : forall lc l' ps' cs' lc' F bid tmn' gl l0 TD 
@@ -309,13 +853,12 @@ Lemma wf_defs_br_uncond : forall lc l' ps' cs' lc' F bid tmn' gl l0 TD
   (H1 : switchToNewBasicBlock TD Mem0 (block_intro l' ps' cs' tmn')
          (block_intro l3 ps3 (cs3' ++ nil) (insn_br_uncond bid l0)) gl lc =
        ret lc')
-  (t : atoms)
-  (Hinscope1 : wf_defs F lc (AtomSetImpl.elements t))
-  (ids0' : atoms)
-  (HeqR12 : AtomSetImpl.diff ids0' (getPhiNodesIDs' ps')[<=]t),
-  wf_defs F lc' (AtomSetImpl.elements ids0').
+  (t : list atom)
+  (Hinscope1 : wf_defs F lc t)
+  (ids0' : list atom)
+  (HeqR12 : incl (ListSet.set_diff eq_atom_dec ids0' (getPhiNodesIDs' ps')) t),
+  wf_defs F lc' ids0'.
 Admitted.
-
 
 Lemma wf_system__wf_insn : forall l1 ps1 cs1 tmn1 f ps los nts s ifs,
   blockInFdefB (block_intro l1 ps1 cs1 tmn1) f = true -> 
@@ -324,6 +867,101 @@ Lemma wf_system__wf_insn : forall l1 ps1 cs1 tmn1 f ps los nts s ifs,
   wf_system ifs s ->
   wf_insn ifs s (module_intro los nts ps) f (block_intro l1 ps1 cs1 tmn1) 
     (insn_terminator tmn1).
+Admitted.
+
+(** * Correctness of reachability analysis *)
+
+(** The entry point of the function is reachable. *)
+
+Lemma reachable_entrypoint:
+  forall (f:fdef) l0 ps cs tmn, 
+    LLVMlib.getEntryBlock f = Some (block_intro l0 ps cs tmn) ->
+    (reachable f)!!l0 = true.
+Proof.
+  intros f l0 ps cs tmn Hentry. unfold reachable.
+  caseEq (reachable_aux f).
+    unfold reachable_aux; intros reach A.
+    rewrite Hentry in A.
+    assert (LBoolean.ge reach!!l0 true).
+      eapply ReachDS.fixpoint_entry. eexact A. auto with coqlib.
+    unfold LBoolean.ge in H. tauto.
+
+    intros. apply AMap.gi.
+Qed.
+
+(** The successors of a reachable instruction are reachable. *)
+
+Lemma reachable_successors:
+  forall f l0 cs ps tmn l1,
+  uniqFdef f ->
+  blockInFdefB (block_intro l0 cs ps tmn) f ->
+  In l1 (successors_terminator tmn) ->
+  (reachable f)!!l0 = true ->
+  (reachable f)!!l1 = true.
+Proof.
+  intros f l0 cs ps tmn l1 HuniqF HbInF Hin.
+  unfold reachable.
+  caseEq (reachable_aux f).
+    unfold reachable_aux. intro reach; intros.
+    remember (LLVMlib.getEntryBlock f) as R.
+    destruct R; inv H.
+    destruct b as [le ? ? ?].
+    assert (LBoolean.ge reach!!l1 reach!!l0) as J.
+      change (reach!!l0) with ((fun pc r => r) l0 (reach!!l0)).
+      eapply ReachDS.fixpoint_solution; eauto.
+        destruct f as [? bs]. simpl in *.
+        clear - HuniqF HbInF Hin.
+        assert ((successors_terminator tmn) = (successors_blocks bs) !!! l0) 
+          as EQ.
+          induction bs.
+            inversion HbInF.
+  
+            assert (J:=HuniqF).
+            simpl_env in J.
+            apply uniqBlocks_inv in J.
+            destruct J as [J1 J2]. 
+            simpl in *.
+            apply orb_prop in HbInF.
+            destruct a.
+            destruct HbInF as [HbInF | HbInF].
+              unfold blockEqB in HbInF.
+              apply sumbool2bool_true in HbInF. inv HbInF.
+              unfold successors_list.
+              rewrite ATree.gss. auto.
+  
+              apply IHbs in J2; auto.
+              unfold successors_list in *.
+              destruct HuniqF as [J _].
+              inv J.
+              rewrite ATree.gso; auto.
+                clear - HbInF H1. admit.
+          rewrite <- EQ; auto.            
+    elim J; intro. congruence. auto.
+
+  intros. apply AMap.gi.
+Qed.
+
+Lemma wf_system__uniqFdef : forall ifs S los nts Ps f,
+  wf_system ifs S -> 
+  moduleInSystemB (module_intro los nts Ps) S = true ->
+  InProductsB (product_fdef f) Ps = true ->
+  uniqFdef f.
+Admitted.
+
+Lemma wf_system__wf_block : forall b f ps los nts s ifs,
+  blockInFdefB b f = true -> 
+  InProductsB (product_fdef f) ps = true ->
+  moduleInSystemB (module_intro los nts ps) s = true ->
+  wf_system ifs s ->
+  wf_block ifs s (module_intro los nts ps) f b.
+Admitted.
+
+Lemma wf_system__uniq_block : forall b f ps los nts s ifs,
+  blockInFdefB b f = true -> 
+  InProductsB (product_fdef f) ps = true ->
+  moduleInSystemB (module_intro los nts ps) s = true ->
+  wf_system ifs s ->
+  NoDup (getBlockIDs b).
 Admitted.
 
 Lemma preservation : forall S1 S2 tr,
@@ -335,10 +973,10 @@ Focus.
 Case "dsReturn".
   destruct HwfS1 as 
     [HwfSystem [HmInS [
-     [HBinF1 [HFinPs1 [Hinscope1 [l1 [ps1 [cs1' Heq1]]]]]] 
+     [Hreach1 [HBinF1 [HFinPs1 [Hinscope1 [l1 [ps1 [cs1' Heq1]]]]]]] 
      [
        [
-         [HBinF2 [HFinPs2 [Hinscope2 [l2 [ps2 [cs2' Heq2]]]]]] 
+         [Hreach2 [HBinF2 [HFinPs2 [Hinscope2 [l2 [ps2 [cs2' Heq2]]]]]]]
          [HwfEC HwfCall]
        ]
        HwfCall'
@@ -357,12 +995,23 @@ Case "dsReturn".
     split; auto.
     split; auto.  
     split; auto. 
-    split. 
+    split; auto.
+    split.
     SSCase "1.1".
       destruct cs'; simpl_env in *.
-      clear - HeqR2 Hinscope2 H1 H.
       SSSCase "1.1.1".
-        apply inscope_of_cmd_tmn in HeqR2.
+        assert (~ In (getCmdID c') (getCmdsIDs cs2')) as Hnotin.
+          eapply wf_system__uniq_block with (f:=F') in HwfSystem; eauto.        
+          simpl in HwfSystem.
+          apply NoDup_inv in HwfSystem.
+          destruct HwfSystem as [_ J].
+          apply NoDup_inv in J.
+          destruct J as [J _].
+          rewrite getCmdsIDs_app in J.
+          simpl in J.
+          apply NoDup_last_inv in J. auto.
+        clear - HeqR2 Hinscope2 H1 H HwfSystem Hnotin.
+        apply inscope_of_cmd_tmn in HeqR2; auto.
         destruct HeqR2 as [ids2 [J1 J2]].        
         rewrite <- J1.
         remember (getCmdID' c') as R.
@@ -372,13 +1021,22 @@ Case "dsReturn".
           destruct n; inv HeqR.
           remember (getOperandValue (los,nts) Mem' Result lc gl) as R1.
           destruct R1; inv H1.
+          (* ?! how to know if g is well-typed!. *)
           eapply wf_defs_updateAddAL; eauto.
 
           destruct n; inv HeqR. inv H1.
           eapply wf_defs_eq; eauto. 
         
       SSSCase "1.1.2".
-        apply inscope_of_cmd_cmd in HeqR2.
+        assert (NoDup (getCmdsIDs (cs2' ++ [c'] ++ [c] ++ cs'))) as Hnodup.
+          eapply wf_system__uniq_block with (f:=F') in HwfSystem; eauto.        
+          simpl in HwfSystem.
+          apply NoDup_inv in HwfSystem.
+          destruct HwfSystem as [_ J].
+          apply NoDup_inv in J.
+          destruct J as [J _]. auto.
+        clear - HeqR2 Hinscope2 H1 H HwfSystem Hnodup.
+        apply inscope_of_cmd_cmd in HeqR2; auto.
         destruct HeqR2 as [ids2 [J1 J2]].        
         rewrite <- J1.
         remember (getCmdID' c') as R.
@@ -401,10 +1059,10 @@ Focus.
 Case "dsReturnVoid".
   destruct HwfS1 as 
     [HwfSystem [HmInS [
-     [HBinF1 [HFinPs1 [Hinscope1 [l1 [ps1 [cs1' Heq1]]]]]] 
+     [Hreach1 [HBinF1 [HFinPs1 [Hinscope1 [l1 [ps1 [cs1' Heq1]]]]]]] 
      [
        [
-         [HBinF2 [HFinPs2 [Hinscope2 [l2 [ps2 [cs2' Heq2]]]]]] 
+         [Hreach2 [HBinF2 [HFinPs2 [Hinscope2 [l2 [ps2 [cs2' Heq2]]]]]]]
          [HwfEC HwfCall]
        ]
        HwfCall'
@@ -423,27 +1081,47 @@ Case "dsReturnVoid".
     split; auto.
     split; auto.
     split; auto.
+    split; auto.
     split.   
     SSCase "1.1".
+      apply HwfCall' in HBinF1. simpl in HBinF1.
       destruct cs'; simpl_env in *.
-      clear - HeqR2 Hinscope2 H HwfCall'.
       SSSCase "1.1.1".
-        apply inscope_of_cmd_tmn in HeqR2.
+        assert (~ In (getCmdID c') (getCmdsIDs cs2')) as Hnotin.
+          eapply wf_system__uniq_block with (f:=F') in HwfSystem; eauto.        
+          simpl in HwfSystem.
+          apply NoDup_inv in HwfSystem.
+          destruct HwfSystem as [_ J].
+          apply NoDup_inv in J.
+          destruct J as [J _].
+          rewrite getCmdsIDs_app in J.
+          simpl in J.
+          apply NoDup_last_inv in J. auto.
+        clear - HeqR2 Hinscope2 H HwfCall' HBinF1 Hnotin.
+        apply inscope_of_cmd_tmn in HeqR2; auto.
         destruct HeqR2 as [ids2 [J1 J2]].        
         rewrite <- J1.
         remember (getCmdID' c') as R.
         destruct c'; try solve [inversion H].
-        destruct n; inversion HwfCall'.
+        destruct n; inversion HBinF1.
         simpl in HeqR. subst R.
         eapply wf_defs_eq; eauto. 
         
       SSSCase "1.1.2".
-        apply inscope_of_cmd_cmd in HeqR2.
+        assert (NoDup (getCmdsIDs (cs2' ++ [c'] ++ [c] ++ cs'))) as Hnodup.
+          eapply wf_system__uniq_block with (f:=F') in HwfSystem; eauto.        
+          simpl in HwfSystem.
+          apply NoDup_inv in HwfSystem.
+          destruct HwfSystem as [_ J].
+          apply NoDup_inv in J.
+          destruct J as [J _]. auto.
+        clear - HeqR2 Hinscope2 H HwfCall' HBinF1 Hnodup.
+        apply inscope_of_cmd_cmd in HeqR2; auto.
         destruct HeqR2 as [ids2 [J1 J2]].        
         rewrite <- J1.
         remember (getCmdID' c') as R.
         destruct c'; try solve [inversion H].
-        destruct n; inversion HwfCall'.
+        destruct n; inversion HBinF1.
         simpl in HeqR. subst R.
         eapply wf_defs_eq; eauto. 
 
@@ -456,8 +1134,8 @@ Focus.
 Case "dsBranch".
   destruct HwfS1 as 
     [HwfSystem [HmInS [
-     [HBinF1 [HFinPs1 [Hinscope1 [l3 [ps3 [cs3' Heq1]]]]]] 
-     [HwfEC _]]]
+     [Hreach1 [HBinF1 [HFinPs1 [Hinscope1 [l3 [ps3 [cs3' Heq1]]]]]]]
+     [HwfEC HwfCall]]]
     ]; subst.
   remember (inscope_of_tmn F
              (block_intro l3 ps3 (cs3' ++ nil)(insn_br bid Cond l1 l2))
@@ -467,11 +1145,36 @@ Case "dsBranch".
   split; auto.
   split; auto.
   SCase "1".
+    split.
+      clear - Hreach1 H0 HBinF1 HFinPs1 HmInS HwfSystem.
+      eapply wf_system__uniqFdef in HwfSystem; eauto.
+      unfold isReachableFromEntry in *.
+      destruct (isGVZero (los, nts) c).
+        symmetry in H0.
+        apply lookupBlockViaLabelFromFdef_inv in H0; eauto.
+        destruct H0 as [H0 _].
+        eapply reachable_successors; eauto.
+          simpl. auto.
+      
+        symmetry in H0.
+        apply lookupBlockViaLabelFromFdef_inv in H0; eauto.
+        destruct H0 as [H0 _].
+        eapply reachable_successors; eauto.
+          simpl. auto.
     split. 
-      clear - H0. admit. (* static *)
+      clear - H0 HBinF1 HFinPs1 HmInS HwfSystem.
+      eapply wf_system__uniqFdef with (f:=F) in HwfSystem; eauto.
+      destruct (isGVZero (los, nts) c).
+        symmetry in H0.
+        apply lookupBlockViaLabelFromFdef_inv in H0; auto.
+          destruct H0; auto.
+        symmetry in H0.
+        apply lookupBlockViaLabelFromFdef_inv in H0; auto.
+          destruct H0; auto.
     split; auto.
     split.
-      clear - H0 HeqR1 H1 Hinscope1 H.
+      eapply wf_system__uniqFdef with (f:=F) in HwfSystem; eauto.
+      clear - H0 HeqR1 H1 Hinscope1 H HwfSystem HBinF1.
       eapply inscope_of_tmn_br in HeqR1; eauto.
       destruct HeqR1 as [ids0' HeqR1].
       destruct cs'.
@@ -484,16 +1187,14 @@ Case "dsBranch".
         eapply wf_defs_br; eauto.
 
       exists l'. exists ps'. exists nil. simpl_env. auto.
-  split; auto.
-    admit. (* need a stronger wf_call that considers rets at all blocks *)    
 Unfocus.
 
 Focus.
 Case "dsBranch_uncond".
   destruct HwfS1 as 
     [HwfSystem [HmInS [
-     [HBinF1 [HFinPs1 [Hinscope1 [l3 [ps3 [cs3' Heq1]]]]]] 
-     [HwfEC _]]]
+     [Hreach1 [HBinF1 [HFinPs1 [Hinscope1 [l3 [ps3 [cs3' Heq1]]]]]]] 
+     [HwfEC HwfCall]]]
     ]; subst.
   remember (inscope_of_tmn F
              (block_intro l3 ps3 (cs3' ++ nil)(insn_br_uncond bid l0))
@@ -501,12 +1202,27 @@ Case "dsBranch_uncond".
   destruct R1; try solve [inversion Hinscope1].
   split; auto.
   split; auto.
-  split; auto.
   SCase "1".
-    split. clear - H0. admit. (* static *)
     split; auto.
     split.
-      clear - H0 HeqR1 Hinscope1 H.
+      clear - Hreach1 H HBinF1 HFinPs1 HmInS HwfSystem.
+      eapply wf_system__uniqFdef with (f:=F) in HwfSystem; eauto.
+      unfold isReachableFromEntry in *.
+      symmetry in H.
+      apply lookupBlockViaLabelFromFdef_inv in H; auto.
+      destruct H as [H _].
+      eapply reachable_successors; eauto.
+        simpl. auto.
+    split.
+      clear - H HBinF1 HFinPs1 HmInS HwfSystem.
+      eapply wf_system__uniqFdef with (f:=F) in HwfSystem; eauto.
+      symmetry in H.
+      apply lookupBlockViaLabelFromFdef_inv in H; auto.
+        destruct H; auto.
+    split; auto.
+    split.
+      eapply wf_system__uniqFdef with (f:=F) in HwfSystem; eauto.
+      clear - H0 HeqR1 Hinscope1 H HwfSystem HBinF1.
       eapply inscope_of_tmn_br_uncond with (cs':=cs')(l':=l')(ps':=ps')
         (tmn':=tmn') in HeqR1; eauto.
       destruct HeqR1 as [ids0' HeqR1].
@@ -520,15 +1236,13 @@ Case "dsBranch_uncond".
         eapply wf_defs_br_uncond; eauto.
 
       exists l'. exists ps'. exists nil. simpl_env. auto.
-  split; auto.
-    admit. (* need a stronger wf_call that considers rets at all blocks *)    
 Unfocus.
 
 Focus.
 Case "dsBop".
   destruct HwfS1 as 
     [HwfSystem [HmInS [
-     [HBinF1 [HFinPs1 [Hinscope1 [l3 [ps3 [cs3' Heq1]]]]]]
+     [Hreach1 [HBinF1 [HFinPs1 [Hinscope1 [l3 [ps3 [cs3' Heq1]]]]]]]
      [HwfEC HwfCall]]]
     ]; subst.
   remember (inscope_of_cmd F
@@ -541,19 +1255,38 @@ Case "dsBop".
   SCase "1".
     split; auto.
     split; auto.
+    split; auto.
     split.  
     SSCase "1.1".
       destruct cs; simpl_env in *.
-      clear - HeqR1 Hinscope1 H.
       SSSCase "1.1.1".
-        apply inscope_of_cmd_tmn in HeqR1.
+        assert (~ In id0 (getCmdsIDs cs3')) as Hnotin.
+          eapply wf_system__uniq_block with (f:=F) in HwfSystem; eauto.        
+          simpl in HwfSystem.
+          apply NoDup_inv in HwfSystem.
+          destruct HwfSystem as [_ J].
+          apply NoDup_inv in J.
+          destruct J as [J _].
+          rewrite getCmdsIDs_app in J.
+          simpl in J.
+          apply NoDup_last_inv in J. auto.
+        clear - HeqR1 Hinscope1 H Hnotin.
+        apply inscope_of_cmd_tmn in HeqR1; auto.
         destruct HeqR1 as [ids2 [J1 J2]].        
         rewrite <- J1.
         apply BOP_inversion in H.
         admit. (* need to prove that gv3 is wf-typed. *)
         
       SSSCase "1.1.2".
-        apply inscope_of_cmd_cmd in HeqR1.
+        assert (NoDup (getCmdsIDs (cs3' ++ [insn_bop id0 bop0 sz0 v1 v2] ++ [c] 
+          ++ cs))) as Hnodup.
+          eapply wf_system__uniq_block with (f:=F) in HwfSystem; eauto.        
+          simpl in HwfSystem.
+          apply NoDup_inv in HwfSystem.
+          destruct HwfSystem as [_ J].
+          apply NoDup_inv in J.
+          destruct J as [J _]. auto.
+        apply inscope_of_cmd_cmd in HeqR1; auto.
         destruct HeqR1 as [ids2 [J1 J2]].        
         rewrite <- J1.
         admit. (* need to prove that gv3 is wf-typed. *)
@@ -587,17 +1320,21 @@ Case "dsCall".
   split; auto.
   split.
   SCase "1".
-    split. admit. (* static *)
-    split. admit. (* static *)
-    split.  
+    split.
+      simpl. eapply reachable_entrypoint; eauto.
+    split.
+      apply entryBlockInFdef in H0; auto.
+    split.
+      eapply lookupFdefViaGV_inv; eauto.
+    split.
       admit. (* need to prove that initial state is good! *)
     exists l'. exists ps'. exists nil. simpl_env. auto.
   split.
   SCase "2".
     split; auto.
   SCase "3".
-    simpl.  
-    destruct tmn'; auto.
+    simpl. intros b HbInBs. destruct b.
+    destruct t; auto.
       admit. (* static: void cannot be assigned as a call ret. *)
 Unfocus.
 
@@ -607,7 +1344,7 @@ Qed.
 Lemma state_tmn_typing : forall ifs s m f b tmn1 defs id1 lc,
   wf_insn ifs s m f b (insn_terminator tmn1) ->
   Some defs = inscope_of_tmn f b tmn1 ->
-  wf_defs f lc (AtomSetImpl.elements defs) ->
+  wf_defs f lc defs ->
   In id1 (getInsnOperands (insn_terminator tmn1)) ->
   exists t, exists gv, lookupAL _ lc id1 = Some gv /\ wf_genericvalue gv t.
 Proof.
@@ -637,7 +1374,7 @@ Case "ret".
     intro J2. inversion J2.
   apply H14 in J'. clear H14.
   clear - J J' HwfDefs Hinscope H0.
-  assert (i0 `in` defs) as J1.
+  assert (In i0 defs) as J1.
     admit.
   admit.
 Admitted.
@@ -645,11 +1382,10 @@ Admitted.
 Lemma state_cmd_typing : forall ifs s m f b c defs id1 lc,
   wf_insn ifs s m f b (insn_cmd c) ->
   Some defs = inscope_of_cmd f b c ->
-  wf_defs f lc (AtomSetImpl.elements defs) ->
+  wf_defs f lc defs ->
   In id1 (getInsnOperands (insn_cmd c)) ->
   exists t, exists gv, lookupAL _ lc id1 = Some gv /\ wf_genericvalue gv t.
 Admitted.
-
 
 Lemma wf_system__blockInFdefB__wf_block : forall b f ps los nts s ifs,
   blockInFdefB b f = true -> 
@@ -681,7 +1417,6 @@ Proof.
     inv Hwfops.
     destruct n; inv Hnth; eauto.
 Qed.        
-
 
 Lemma getValueViaLabelFromValuels__getInsnOperands : forall
   (lc : GVMap)
@@ -771,11 +1506,11 @@ Lemma wf_phinodes__getIncomingValuesForBlockFromPHINodes : forall
   (lc : GVMap)
   (gl : GVMap)
   (M : mem)
-  (t : atoms)
+  (t : list atom)
   l1 ps1 cs1
   (HeqR : ret t = inscope_of_tmn f 
     (block_intro l1 ps1 cs1 (insn_br_uncond i0 l0)) (insn_br_uncond i0 l0))
-  (Hinscope : wf_defs f lc (AtomSetImpl.elements t))
+  (Hinscope : wf_defs f lc t)
   (ps' : phinodes)
   (cs' : cmds)
   (tmn' : terminator)
@@ -861,7 +1596,7 @@ Proof.
     admit. (* we should rule out this case. *)
 
   destruct e as [f b cs tmn lc als].
-  destruct HwfECs as [[HbInF [HfInPs [Hinscope [l1 [ps1 [cs1 Heq]]]]]] 
+  destruct HwfECs as [[Hreach [HbInF [HfInPs [Hinscope [l1 [ps1 [cs1 Heq]]]]]]] 
                       [HwfECs HwfCall]].
   subst b.
   destruct cs.
@@ -876,13 +1611,15 @@ Proof.
 
         right.
         destruct e as [f' b' cs' tmn' lc' als'].
-        destruct cs'; try solve [inversion HwfCall].
-        destruct c; try solve [inversion HwfCall]. clear HwfCall.
+        assert (J:=HbInF).
+        apply HwfCall in J. clear HwfCall.
+        destruct cs'; try solve [inversion J].
+        destruct c; try solve [inversion J]. clear J.
         assert (exists M', free_allocas (los,nts) M als = Some M') as J.
           admit.
         destruct J as [M' J].
         assert (exists lc'', 
-          returnUpdateLocals (los,nts) M' (insn_call i1 n t1 t2 v0 p) v lc lc' gl
+          returnUpdateLocals (los,nts) M' (insn_call i1 n t0 t1 v0 p) v lc lc' gl
             = Some lc'') as Hretup.
           unfold returnUpdateLocals. simpl.
           destruct n.
@@ -894,7 +1631,7 @@ Proof.
               assert (exists t, exists gv, lookupAL _ lc vid = Some gv /\ 
                 wf_genericvalue gv t) as Hlkup.
                 assert (In vid (getInsnOperands (insn_terminator 
-                  (insn_return i0 t0 (value_id vid))))) as HinOps.
+                  (insn_return i0 t (value_id vid))))) as HinOps.
                   simpl. auto.
                 eapply state_tmn_typing in HwfInstr; eauto.
 
@@ -917,13 +1654,13 @@ Proof.
     SCase "tmn=br_uncond". 
       right.
       assert (exists ps', exists cs', exists tmn',
-        Some (block_intro l0 ps' cs' tmn') = lookupBlockViaLabelFromFdef f l0) 
+        Some (block_intro l2 ps' cs' tmn') = lookupBlockViaLabelFromFdef f l2) 
           as HlkB.
         admit. (* wf *)
       destruct HlkB as [ps' [cs' [tmn' HlkB]]].
       assert (exists RVs, 
         getIncomingValuesForBlockFromPHINodes (los, nts) M ps'
-          (block_intro l1 ps1 (cs1 ++ nil) (insn_br_uncond i0 l0)) gl lc =
+          (block_intro l1 ps1 (cs1 ++ nil) (insn_br_uncond i0 l2)) gl lc =
         Some RVs) as J.
         eapply wf_system__blockInFdefB__wf_block in HbInF; eauto.
         eapply wf_system__lookup__wf_block in HlkB; eauto.
@@ -934,15 +1671,15 @@ Proof.
 
       destruct J as [RVs J].
       assert (exists lc', switchToNewBasicBlock (los, nts) M
-        (block_intro l0 ps' cs' tmn') 
-        (block_intro l1 ps1 (cs1 ++ nil) (insn_br_uncond i0 l0)) gl lc = 
+        (block_intro l2 ps' cs' tmn') 
+        (block_intro l1 ps1 (cs1 ++ nil) (insn_br_uncond i0 l2)) gl lc = 
           Some lc') as Hswitch.
         unfold switchToNewBasicBlock. simpl.
         rewrite J. 
         exists (updateValuesForNewBlock RVs lc). auto.
       destruct Hswitch as [lc' Hswitch].
       exists (mkState s (los, nts) ps 
-              ((mkEC f (block_intro l0 ps' cs' tmn') cs' tmn' lc' als)
+              ((mkEC f (block_intro l2 ps' cs' tmn') cs' tmn' lc' als)
               ::ecs) gl fs M).
       exists trace_nil. eauto.
 
